skeleton of proof with generalized IH

theories/type_checker_reflects_typing.v
@@ -5,12 +5,13 @@ From mathcomp Require Import ssreflect ssrfun ssrnat ssrbool eqtype seq.
 
 Require Import Coq.Program.Equality.
 
+Require Import Lia.
+
 Set Implicit Arguments.
 Unset Strict Implicit.
 Unset Printing Implicit Defensive.
 
-From Wasm Require Import common operations typing type_checker.
-
+From Wasm Require Import common operations typing type_checker properties.
 
 Section Host.
 
@@ -27,14 +28,12 @@ Proof.
   - apply: Bool.ReflectT. by constructor.
 Qed.
 
-
 Lemma ct_suffix_empty: forall l,
     ct_suffix [::] l.
 Proof.
   move => l. unfold ct_suffix => /=.
   rewrite subn0. apply/eqP. by apply drop_size.
 Qed.
-
 
 Lemma upd_label_overwrite: forall C loc lab ret lab',
   upd_label (upd_local_label_return C loc lab ret) lab'
@@ -52,15 +51,122 @@ Ltac bool_to_prop_and:=
            move/andP in H; destruct H
          | H: _ && _ |- _ =>
            move/andP in H; destruct H
-end.
+         end.
+
+Ltac simplify_hypothesis Hb :=
+  repeat match type of Hb with
+  | is_true (es_is_trap _) => move/es_is_trapP: Hb => Hb
+  | ?b = true => fold (is_true b) in Hb
+  | (_ == _) = false => move/eqP in Hb
+  | context C [size (rev _)] => rewrite size_rev in Hb
+  | context C [take _ (rev _)] => rewrite take_rev in Hb
+  | context C [rev (rev _)] => rewrite revK in Hb
+  | context C [true && _] => rewrite Bool.andb_true_l in Hb
+  | context C [_ && true] => rewrite Bool.andb_true_r in Hb
+  | context C [false || _] => rewrite Bool.orb_false_l in Hb
+  | context C [_ || false] => rewrite Bool.orb_false_r in Hb
+  | context C [type_update _ _] => unfold type_update in Hb; simpl in Hb
+  | context C [ct_suffix [::] _] => rewrite ct_suffix_empty in Hb; simpl in Hb
+  | context C [?x - 0] => rewrite subn0 in Hb; simpl in Hb
+  | context C [take (size ?x) ?x] => rewrite take_size in Hb; simpl in Hb
+  | context C [produce _ _] => unfold produce in Hb; simpl in Hb
+  | exists _, _ /\ _ => destruct Hb as [tx [Hsuffix Hbet]]
+  | is_true true => clear Hb
+  | is_true false => exfalso; apply: notF; apply: Hb
+  | is_true (_ == _) => move/eqP in Hb
+  | ?x = ?x => clear Hb
+  | _ = _ => rewrite Hb in *
+         end.
+
+Ltac simplify_goal :=
+  repeat match goal with H: _ |- _ => progress simplify_hypothesis H end.
+
+Lemma CT_top_empty_consume: forall tf,
+  consume (CT_top_type [::]) tf = CT_top_type [::].
+Proof.
+  move => tf. unfold consume.
+  destruct tf => //=.
+  by rewrite ct_suffix_empty.
+Qed.
+
+Fixpoint populate_ct_aux (l: list checker_type_aux): list value_type :=
+  match l with
+  | [::] => [::]
+  | t :: l' =>
+    match t with
+    | CTA_any => T_i32
+    | CTA_some vt => vt
+    end
+      :: populate_ct_aux l'
+  end.
+
+Definition populate_ct (ct: checker_type) : list value_type :=
+  match ct with
+  | CT_type tn => tn
+  | CT_top_type tn => populate_ct_aux tn
+  | CT_bot => [::]
+  end.
+
+Lemma populate_ct_aux_suffix: forall l,
+  ct_suffix l (to_ct_list (populate_ct_aux l)).
+Proof.
+Admitted.
+  
+Lemma populate_ct_agree: forall l,
+  c_types_agree l (populate_ct l).
+Proof.
+Admitted.
+
+Lemma tc_to_bet_generalized: forall C bes tm ct,
+  (match List.fold_left (check_single C) bes ct with
+        | CT_top_type ts => ct_suffix ts (to_ct_list tm)
+        | CT_type ts => ts == tm
+        | CT_bot => false end) = true -> 
+  match ct with 
+  | CT_type tn => be_typing C bes (Tf tn tm)
+  | CT_top_type tn => exists tn', c_types_agree (CT_top_type tn) tn' /\ be_typing C bes (Tf tn' tm)
+  | CT_bot => true
+  end.
+Proof.
+  move => C bes. move: C.
+  elim: bes => //=.
+  - move => C tm ct.
+    destruct ct => //=.
+    + move => Hsuffix.
+      exists tm.
+      split => //=.
+      replace tm with (tm ++ [::]); last by apply cats0.
+      apply bet_weakening.
+      by apply bet_empty.
+    + move => Heq.
+      move/eqP in Heq. subst.
+      replace tm with (tm ++ [::]); last by apply cats0.
+      apply bet_weakening.
+      by apply bet_empty.
+  - move => be bes IH C tm ct Htc.
+    apply IH in Htc.
+    destruct ct, be => //=; simpl in Htc; simplify_hypothesis Htc.
+    (* 56 cases *)
+    + exists (populate_ct_aux l).
+      split; first by apply populate_ct_aux_suffix.
+      eapply bet_composition_front; last by apply Hbet.
+      by apply bet_unreachable.
+Admitted.
+  
+Lemma b_e_type_checker_reflects_typing:
+  forall C bes tf,
+    reflect (be_typing C bes tf) (b_e_type_checker C bes tf).
+Proof.
+  move => C bes tf.
+  destruct tf as [tn tm].
+  destruct (b_e_type_checker C bes (Tf tn tm)) eqn: Htc_bool.
+  - apply ReflectT.
+    unfold b_e_type_checker, c_types_agree in Htc_bool.
+    by apply tc_to_bet_generalized in Htc_bool.
+  - admit.  
+Admitted.
+    
 (*
-
-(* 
-  This seems really non-trivial. The structure might also change after we fix
-    the duplication in the definition of be_type_check. How about we leave this
-    as admitted for now and explore other things first?
-*)
-
 Lemma wasm_type_checker_reflects_typing:
   forall C cl,
     reflect (cl_typing_self C cl) (cl_type_check C cl).
@@ -114,9 +220,7 @@ Proof.
       
 
     
-Admitted. (* TODO *)
-
+Admitted.
 *)
-
 End Host.
 
